feat: proof mode instances for telescopes (#659)
---------

Co-authored-by: Michael Sammler <noreply@sammler.me>

Iris/Iris/Std/Telescopes.lean
@@ -6,6 +6,8 @@ Authors: Markus de Medeiros
 module
 
 public import Iris.Init
+public import Iris.Std.DelabRule
+public import Iris.Std.Notation
 
 /-!
 # Telescopes
@@ -19,6 +21,7 @@ a block of binders.
 @[expose] public section
 
 namespace Iris.Std
+open Iris.Std Lean PrettyPrinter Delaborator
 
 universe u v
 
@@ -66,6 +69,60 @@ one binder at a time. -/
 def fold {B : Type v} (step : (A : Type u) → (A → B) → B) : {TT : Tele.{u}} → (TT -t> B) → B
   | .nil, f => ULift.down f
   | .cons _, f => step _ fun x => fold step (f x)
+
+/-- Telescopic universal quantification at `Prop`. -/
+def tforall : {TT : Tele.{u}} → (TT.Arg → Prop) → Prop
+  | .nil,    Ψ => Ψ .nil
+  | .cons _, Ψ => ∀ x, tforall fun xs => Ψ (.cons x xs)
+
+/-- Telescopic existential quantification at `Prop`. -/
+def texist : {TT : Tele.{u}} → (TT.Arg → Prop) → Prop
+  | .nil,    Ψ => Ψ .nil
+  | .cons _, Ψ => ∃ x, texist fun xs => Ψ (.cons x xs)
+
+/-- Telescopic universal quantification. -/
+macro "∀.." xs:explicitBinders ", " P:term : term => do
+  return ⟨← expandExplicitBinders ``tforall xs P⟩
+
+/-- Telescopic existential quantification. -/
+macro "∃.." xs:explicitBinders ", " P:term : term => do
+  return ⟨← expandExplicitBinders ``texist xs P⟩
+
+/-- A delaborator for the telescopic universal quantifier. -/
+@[app_delab Iris.Std.Tele.tforall]
+meta def delabPropTforall : Delab :=
+  delabQuant 2 pure
+    (fun x rest body => `(∀.. $x:ident $[$rest:ident]*, $body))
+    (fun | `(∀.. $y:ident $[$z:ident]*, $Ψ) => some (y, z, Ψ) | _ => none)
+
+/-- A delaborator for the telescopic existential quantifier. -/
+@[app_delab Iris.Std.Tele.texist]
+meta def delabPropTexist : Delab := do
+  delabQuant 2 pure
+    (fun x rest body => `(∃.. $x:ident $[$rest:ident]*, $body))
+    (fun | `(∃.. $y:ident $[$z:ident]*, $Ψ) => some (y, z, Ψ) | _ => none)
+
+theorem tforall_forall {TT : Tele} (Ψ : TT.Arg → Prop) : tforall Ψ ↔ ∀ x, Ψ x := by
+  induction TT with
+  | nil =>
+    constructor
+    · exact fun h _ => h
+    · exact fun h => h .nil
+  | cons b ih =>
+    constructor
+    · exact fun h x => (ih x.fst _).mp (h x.fst) x.snd
+    · exact fun h x => (ih x _).mpr fun xs => h ⟨x, xs⟩
+
+theorem texist_exist {TT : Tele} (Ψ : TT.Arg → Prop) : texist Ψ ↔ ∃ x, Ψ x := by
+  induction TT with
+  | nil =>
+    constructor
+    · exact fun h => ⟨.nil, h⟩
+    · exact fun ⟨_, h⟩ => h
+  | cons b ih =>
+    constructor
+    · exact fun ⟨x, h⟩ => let ⟨xs, h⟩ := (ih x _).mp h; ⟨⟨x, xs⟩, h⟩
+    · exact fun ⟨x, h⟩ => ⟨x.fst, (ih x.fst _).mpr ⟨x.snd, h⟩⟩
 
 end Tele
 
